proof/refine/ARM/Interrupt_R.thy
@@ -50,6 +50,8 @@ primrec
 where
   "arch_irq_control_inv_relation (ARM_A.ArchIRQControlIssue i ptr1 ptr2 t) x =
      (x = ARM_H.IssueIRQHandler i (cte_map ptr1) (cte_map ptr2) t)"
+| "arch_irq_control_inv_relation (ARM_A.IssueSGISignal irq target ptr ptr') x =
+     (x = ARM_H.IssueSGISignal (ucast irq) (ucast target) (cte_map ptr) (cte_map ptr'))"
 
 primrec
   irq_control_inv_relation :: "irq_control_invocation \<Rightarrow> irqcontrol_invocation \<Rightarrow> bool"
@@ -79,6 +81,10 @@ where
                  cte_wp_at' (\<lambda>cte. cteCap cte = IRQControlCap) p' and
                  ex_cte_cap_to' p and real_cte_at' p and
                 (Not o irq_issued' irq) and K (irq \<le> maxIRQ))"
+| "arch_irq_control_inv_valid' (ARM_H.IssueSGISignal irq target src_slot sgi_slot) =
+     (cte_wp_at' (\<lambda>cte. cteCap cte = NullCap) sgi_slot and
+      cte_wp_at' (\<lambda>cte. cteCap cte = IRQControlCap) src_slot and
+      ex_cte_cap_to' sgi_slot and real_cte_at' sgi_slot)"
 
 primrec
   irq_control_inv_valid' :: "irqcontrol_invocation \<Rightarrow> kernel_state \<Rightarrow> bool"
@@ -196,6 +202,22 @@ lemma arch_check_irq_maxIRQ_valid':
   "\<lbrace>\<top>\<rbrace> arch_check_irq irq \<lbrace>\<lambda>_ _. irq \<le> Kernel_Config.maxIRQ\<rbrace>, \<lbrace>\<lambda>_. \<top>\<rbrace>"
   by (wp arch_check_irq_maxIRQ_valid)
 
+lemma isSGITargetValid_eq:
+  "isSGITargetValid w = sgi_target_valid w"
+  unfolding isSGITargetValid_def sgi_target_valid_def
+  by simp
+
+lemma sgi_target_cast[simp]:
+  "sgi_target_valid w \<Longrightarrow> ucast (ucast w :: sgi_target) = w"
+  unfolding sgi_target_valid_def gicNumTargets_def
+  by (simp flip: sgi_target_len_def add: ucast_ucast_len sgi_target_len_val)
+
+lemma sgi_irq_cast:
+  "w \<le> word_of_nat numSGIs - 1 \<Longrightarrow> ucast (ucast w :: sgi_irq) = (w :: machine_word)"
+  unfolding numSGIs_def
+  by (simp flip: sgi_irq_len_def
+           add: ucast_ucast_len sgi_irq_len_val word_le_nat_alt word_less_nat_alt)
+
 lemma arch_decodeIRQControlInvocation_corres:
   "list_all2 cap_relation caps caps' \<Longrightarrow>
    corres (ser \<oplus> arch_irq_control_inv_relation)
@@ -212,11 +234,18 @@ lemma arch_decodeIRQControlInvocation_corres:
                  simp: length_Suc_conv list_all2_Cons1 whenE_rangeCheck_eq liftE_bindE split_def)[2]
   apply (cases caps, simp split: list.split)
   apply (case_tac "\<exists>n. length args = Suc (Suc (Suc (Suc n)))",
-              clarsimp simp: length_Suc_conv list_all2_Cons1 whenE_rangeCheck_eq
-                             liftE_bindE split_def)
+              clarsimp simp: length_Suc_conv list_all2_Cons1 liftE_bindE split_def)
    prefer 2 apply (auto split: list.split)[1]
-  \<comment>\<open>ARMIRQIssueIRQHandler\<close>
+  \<comment>\<open>ARMIRQIssueSGISignal\<close>
   apply (rule conjI, clarsimp)
+   apply (simp add: range_check_def rangeCheck_def)
+   apply (corres corres: lookupSlotForCNodeOp_corres ensureEmptySlot_corres corres_returnOkTT
+                 term_simp: numSGIs_def isSGITargetValid_eq sgi_irq_cast)
+    apply fastforce
+   apply fastforce
+  \<comment>\<open>ARMIRQIssueIRQHandler\<close>
+  apply (rule impI, rule conjI, clarsimp)
+  \<comment>\<open>ARMIRQIssueIRQHandler\<close>
    apply (rule corres_guard_imp)
      apply (rule corres_splitEE[OF checkIRQ_corres])
        apply (rule_tac F="y \<le> Kernel_Config.maxIRQ" in corres_gen_asm)
@@ -330,6 +359,7 @@ lemma arch_decode_irq_control_valid'[wp]:
           | wp whenE_throwError_wp isIRQActive_wp ensureEmptySlot_stronger
           | wpc
           | wp (once) hoare_drop_imps)+
+  apply (clarsimp, rule conjI; clarsimp)
   apply (clarsimp simp: invs_valid_objs' toEnum_unat_ucast
                         le_maxIRQ_machine_less_irqBits_val irq_machine_le_maxIRQ_irq)
   done
@@ -495,8 +525,10 @@ lemma IRQHandler_valid':
 crunch setIRQState
   for valid_mdb'[wp]: "valid_mdb'"
 
-lemma no_fail_setIRQTrigger: "no_fail \<top> (setIRQTrigger irq trig)"
-  by (simp add: setIRQTrigger_def)
+lemma no_fail_setIRQTrigger[wp]:
+  "no_fail \<top> (setIRQTrigger irq t)"
+  unfolding setIRQTrigger_def
+  by wpsimp
 
 lemma setIRQTrigger_corres:
   "corres dc \<top> \<top> (do_machine_op (setIRQTrigger irq t)) (doMachineOp (setIRQTrigger irq t))"
@@ -505,12 +537,15 @@ lemma setIRQTrigger_corres:
     apply (rule corres_rel_imp)
      apply (wp
             | rule corres_underlying_trivial
-            | rule no_fail_setIRQTrigger
             | simp add: dc_def)+
   done
 
 crunch set_irq_state
   for valid_arch_state[wp]: valid_arch_state
+
+lemma SGISignalCap_valid[simp, intro!]:
+  "valid_cap' (ArchObjectCap (SGISignalCap irq target)) s"
+  by (simp add: valid_cap'_def capAligned_def word_bits_def)
 
 lemma arch_performIRQControl_corres:
   "arch_irq_control_inv_relation x2 ivk' \<Longrightarrow> corres (dc \<oplus> dc)
@@ -519,23 +554,31 @@ lemma arch_performIRQControl_corres:
           (arch_invoke_irq_control x2)
           (Arch.performIRQControl ivk')"
   apply (cases x2; simp add: ARM_H.performIRQControl_def invoke_irq_control.cases IRQ_def)
-  apply (rule corres_guard_imp)
-    apply (rule corres_split_nor)
-       apply (rule setIRQTrigger_corres)
-      apply (rule corres_split_nor)
-         apply (rule setIRQState_corres)
-         apply (simp add: irq_state_relation_def)
-        apply (rule cteInsert_simple_corres; simp)
-       apply (wp | simp add: irq_state_relation_def IRQHandler_valid IRQHandler_valid')+
+   apply (rule corres_guard_imp)
+     apply (rule corres_split_nor)
+        apply (rule setIRQTrigger_corres)
+       apply (rule corres_split_nor)
+          apply (rule setIRQState_corres)
+          apply (simp add: irq_state_relation_def)
+         apply (rule cteInsert_simple_corres; simp)
+        apply (wp | simp add: irq_state_relation_def IRQHandler_valid IRQHandler_valid')+
+    apply (clarsimp simp: invs_def valid_state_def valid_pspace_def cte_wp_at_caps_of_state
+                          is_simple_cap_def is_cap_simps arch_irq_control_inv_valid_def
+                          safe_parent_for_def)
+   apply (clarsimp simp: invs'_def valid_state'_def valid_pspace'_def IRQHandler_valid
+                         IRQHandler_valid' is_simple_cap'_def isCap_simps IRQ_def)
+   apply (clarsimp simp: safe_parent_for'_def cte_wp_at_ctes_of)
+   apply (rename_tac cte', case_tac cte')
+   apply (clarsimp simp: isCap_simps sameRegionAs_def3)
+   apply (auto dest: valid_irq_handlers_ctes_ofD)[1]
+  apply (corres corres: cteInsert_simple_corres)
    apply (clarsimp simp: invs_def valid_state_def valid_pspace_def cte_wp_at_caps_of_state
                          is_simple_cap_def is_cap_simps arch_irq_control_inv_valid_def
-                         safe_parent_for_def)
-  apply (clarsimp simp: invs'_def valid_state'_def valid_pspace'_def IRQHandler_valid
-                        IRQHandler_valid' is_simple_cap'_def isCap_simps IRQ_def)
+                         safe_parent_for_def is_irq_control_descendant_def)
+  apply (clarsimp simp: invs'_def valid_state'_def valid_pspace'_def
+                        is_simple_cap'_def isCap_simps)
   apply (clarsimp simp: safe_parent_for'_def cte_wp_at_ctes_of)
-  apply (case_tac ctea)
-  apply (clarsimp simp: isCap_simps sameRegionAs_def3)
-  apply (auto dest: valid_irq_handlers_ctes_ofD)[1]
+  apply (rename_tac cte', case_tac cte', simp add: isCap_simps)
   done
 
 lemma performIRQControl_corres:
@@ -600,10 +643,10 @@ lemma arch_invoke_irq_control_invs'[wp]:
           | wpc)+
   apply (clarsimp simp: cte_wp_at_ctes_of IRQHandler_valid' is_simple_cap'_def isCap_simps
                         safe_parent_for'_def sameRegionAs_def3)
-  apply (rule conjI, clarsimp simp: cte_wp_at_ctes_of)
-  apply (case_tac ctea)
-  apply (auto dest: valid_irq_handlers_ctes_ofD
-              simp: invs'_def valid_state'_def IRQ_def)
+  apply (clarsimp simp: capRange_def)
+  apply (rule conjI; clarsimp simp: cte_wp_at_ctes_of; case_tac ctea)
+   apply (auto dest: valid_irq_handlers_ctes_ofD
+               simp: invs'_def valid_state'_def IRQ_def)
   done
 
 lemma invoke_irq_control_invs'[wp]:
