proof/refine/ARM_HYP/Retype_R.thy
@@ -2516,6 +2516,14 @@ lemma descendants_of_retype':
 lemma capRange_Null [simp]: "capRange NullCap = {}"
   by (simp add: capRange_def)
 
+lemma valid_arch_badges_not_arch:
+  "\<not>isArchObjectCap cap' \<Longrightarrow> valid_arch_badges cap cap' node"
+  by (auto simp: isCap_simps valid_arch_badges_def)
+
+lemma valid_arch_badges_NullCap[simp]:
+  "valid_arch_badges cap NullCap node"
+  by (simp add: valid_arch_badges_not_arch isCap_simps)
+
 end
 
 locale retype_mdb = vmdb +
@@ -2621,7 +2629,7 @@ proof -
   have "valid_badges m" ..
   thus ?thesis
     apply (clarsimp simp: valid_badges_def)
-    apply (simp add: n_Some_eq n_next split: if_split_asm)
+    apply (simp add: n_Some_eq n_next isCap_simps split: if_split_asm)
     apply fastforce
     done
 qed
